Preamble file

Token.fst
@@ -1,7 +1,6 @@
 
 (******************)
 module Token
-
 open FStar.All
 open FStar.UInt160
 open FStar.UInt256
@@ -17,53 +16,54 @@ let set #key #vl f ind x ind2 = if ind = ind2 then x else f ind2
 val get : #key:eqtype -> #vl:Type -> (key -> vl) -> key -> vl
 let get #key #vl f ind = f ind
 
-exception EvmThrow
+exception SolidityThrow
+exception SolidityReturn
 
 val do_call : #state:Type -> #ret:Type -> (state -> ML (option ret * state)) -> state -> ML (option ret * state)
 let do_call #state #ret meth st =
   try meth st
-  with EvmThrow -> (None, st)
+  with SolidityThrow -> (None, st)
+
+(*
+
+Could generate this kind of setters and getters in methods:
+
+let balance_set addr x = s := {!s with balance = set (!s).balance addr x } in
+let balance_get addr = get (!s).balance addr in
+
+*)
 
 
 
 
 (* Storage state *)
 noeq type state = {
-balance : (UInt160.t -> UInt256.t);
+balance : UInt160.t -> UInt256.t;
 }
 
-noeq type mut_state = {
-m_balance : ref (UInt160.t -> UInt256.t);
-}
-
-
-let test () =
-  let foo = Some 123 in
-  match foo with
-  | None -> assert False
-  | Some k -> ()
 
 
 (* Contract methods *)
-val method_Token : msg -> mut_state -> UInt256.t -> ML (option unit)
+val method_Token : msg -> state -> UInt256.t -> ML (option (unit) * state)
 let method_Token msg state n =
+let s = alloc state in
 let ret = alloc None in
-state.m_balance := set !(state.m_balance) ((msg).sender) (n);
-!ret
+try
+s := {!s with balance = set (!s).balance ((msg).sender) (n) };
+(!ret, !s)
+with SolidityReturn -> (!ret, !s)
 
 
 val method_send : msg -> state -> UInt160.t -> UInt256.t -> ML (option (unit) * state)
 let method_send msg state a amount =
 let s = alloc state in
-let balance_set addr x = s := {!s with balance = set (!s).balance addr x } in
-let balance_get addr = get (!s).balance addr in
-
 let ret = alloc None in
+try
 if UInt256.lt (get (!s).balance ((msg).sender)) (amount)
-then (raise EvmThrow; ())
+then (raise SolidityThrow; ())
 else ();
-balance_set ((msg).sender) (UInt256.sub_mod (balance_get ((msg).sender)) (amount));
-balance_set (a) (UInt256.add_mod (balance_get (a)) (amount));
+
+s := {!s with balance = set (!s).balance ((msg).sender) (UInt256.sub_mod (get (!s).balance ((msg).sender)) (amount)) };
+s := {!s with balance = set (!s).balance (a) (UInt256.add_mod (get (!s).balance (a)) (amount)) };
 (!ret, !s)
-
-
+with SolidityReturn -> (!ret, !s)
