Preamble.fst
@@ -1,0 +1,32 @@
+open FStar.All
+open FStar.UInt160
+open FStar.UInt256
+open FStar.Heap
+
+type msg = {
+sender : UInt160.t;
+}
+
+val set : #key:eqtype -> #vl:Type -> (key -> vl) -> key -> vl -> (key -> vl)
+let set #key #vl f ind x ind2 = if ind = ind2 then x else f ind2
+
+val get : #key:eqtype -> #vl:Type -> (key -> vl) -> key -> vl
+let get #key #vl f ind = f ind
+
+exception SolidityThrow
+exception SolidityReturn
+
+val do_call : #state:Type -> #ret:Type -> (state -> ML (option ret * state)) -> state -> ML (option ret * state)
+let do_call #state #ret meth st =
+  try meth st
+  with SolidityThrow -> (None, st)
+
+(*
+
+Could generate this kind of setters and getters in methods:
+
+let balance_set addr x = s := {!s with balance = set (!s).balance addr x } in
+let balance_get addr = get (!s).balance addr in
+
+*)
+
